disk-betree/AsyncBlockCache.dfy
@@ -1,0 +1,157 @@
+include "Betree.dfy"
+include "../lib/sequences.dfy"
+include "../lib/Maps.dfy"
+include "Graph.dfy"
+include "AsyncDiskModel.dfy"
+include "BlockCache.dfy"
+
+abstract module AsyncBlockCache refines Transactable {
+  import opened Maps
+  import opened Options
+  import LBAType
+
+  import Disk = AsyncDisk
+
+  type ReqId = Disk.ReqId
+  type LBA = LBAType.LBA
+  datatype Constants = Constants()
+  function method IndirectionTableLBA() : LBA { LBAType.IndirectionTableLBA() }
+
+  // TODO make indirectionTable take up more than one block
+  datatype IndirectionTable = IndirectionTable(
+      lbas: map<Reference, LBA>,
+      graph: map<Reference, seq<Reference>>)
+
+  datatype Sector =
+    | SectorBlock(block: Node)
+    | SectorIndirectionTable(indirectionTable: IndirectionTable)
+
+  type DiskOp = Disk.DiskOp<LBA, Sector>
+
+  // BlockCache stuff
+
+  datatype OutstandingWrite = OutstandingWrite(ref: Reference, lba: LBA)
+  datatype OutstandingRead = OutstandingRead(ref: Reference)
+  datatype OutstandingIndirectionTableWrite = OutstandingIndirectionTableWrite(reqId: ReqId, indirectionTable: IndirectionTable)
+
+  datatype Variables =
+    | Ready(
+        persistentIndirectionTable: IndirectionTable,
+        ephemeralIndirectionTable: IndirectionTable,
+        outstandingIndirectionTableWrite: Option<OutstandingIndirectionTableWrite>,
+        
+        outstandingBlockWrites: map<ReqId, OutstandingWrite>,
+        outstandingBlockReads: map<ReqId, OutstandingRead>,
+
+        cache: map<Reference, Node>)
+    | Unready(outstandingIndirectionTableRead: Option<ReqId>)
+
+  predicate IsAllocated(s: Variables, ref: Reference)
+  requires s.Ready?
+  {
+    ref in s.ephemeralIndirectionTable.graph
+  }
+  predicate ValidLBAForNode(k: Constants, lba: LBA)
+  {
+    lba != IndirectionTableLBA()
+  }
+
+  datatype Step =
+    | WriteBackReqStep(ref: Reference)
+    | WriteBackRespStep
+    | WriteBackIndirectionTableReqStep
+    | WriteBackIndirectionTableRespStep
+    | UnallocStep(ref: Reference)
+    | PageInReqStep(ref: Reference)
+    | PageInRespStep
+    | PageInIndirectionTableReqStep
+    | PageInIndirectionTableRespStep
+    | EvictStep(ref: Reference)
+    | NoOpStep
+    | TransactionStep(ops: seq<Op>)
+
+  predicate WriteBackReq(k: Constants, s: Variables, s': Variables, dop: DiskOp, ref: Reference)
+  {
+    && s.Ready?
+    && dop.ReqWriteOp?
+    && ref in s.cache
+    && ValidLBAForNode(k, dop.reqWrite.lba)
+    && dop.reqWrite.lba !in s.persistentIndirectionTable.lbas.Values
+    && dop.reqWrite.lba !in s.ephemeralIndirectionTable.lbas.Values
+    && dop.reqWrite.sector == SectorBlock(s.cache[ref])
+    && s'.Ready?
+    && s'.persistentIndirectionTable == s.persistentIndirectionTable
+    && s'.ephemeralIndirectionTable.lbas == s.ephemeralIndirectionTable.lbas[ref := dop.reqWrite.lba]
+    && s'.ephemeralIndirectionTable.graph == s.ephemeralIndirectionTable.graph
+    && s'.cache == s.cache
+    && s'.outstandingBlockWrites == s.outstandingBlockWrites[dop.id := OutstandingWrite(ref, dop.reqWrite.lba)]
+    && s'.outstandingBlockReads == s.outstandingBlockReads
+    && s'.outstandingIndirectionTableWrite == s'.outstandingIndirectionTableWrite
+    && s.outstandingIndirectionTableWrite == s.outstandingIndirectionTableWrite
+  }
+
+  predicate WriteBackResp(k: Constants, s: Variables, s': Variables, dop: DiskOp)
+  {
+    && s.Ready?
+    && dop.RespWriteOp?
+    && dop.id in s.outstandingBlockWrites
+    && s' == s.(outstandingBlockWrites := MapRemove1(s.outstandingBlockWrites, dop.id))
+  }
+
+  predicate WriteBackIndirectionTableReq(k: Constants, s: Variables, s': Variables, dop: DiskOp)
+  {
+    && s.Ready?
+    && dop.ReqWriteOp?
+    && dop.reqWrite.lba == IndirectionTableLBA()
+    && dop.reqWrite.sector == SectorIndirectionTable(s.ephemeralIndirectionTable)
+    && s.cache.Keys <= s.ephemeralIndirectionTable.lbas.Keys
+    && s.outstandingIndirectionTableWrite.None?
+    && s.outstandingBlockWrites == map[]
+    && s' == s.(outstandingIndirectionTableWrite := Some(OutstandingIndirectionTableWrite(dop.id, s.ephemeralIndirectionTable)))
+  }
+
+  predicate WriteBackIndirectionTableResp(k: Constants, s: Variables, s': Variables, dop: DiskOp)
+  {
+    && s.Ready?
+    && dop.RespWriteOp?
+    && s.outstandingIndirectionTableWrite.Some?
+    && dop.id == s.outstandingIndirectionTableWrite.value.reqId
+    && s' == s.(outstandingIndirectionTableWrite := None)
+              .(persistentIndirectionTable := s.outstandingIndirectionTableWrite.value.indirectionTable)
+  }
+
+  predicate NoPredecessors(graph: map<Reference, seq<Reference>>, ref: Reference)
+  {
+    forall r | r in graph :: ref !in graph[r]
+  }
+
+  predicate Unalloc(k: Constants, s: Variables, s': Variables, dop: DiskOp, ref: Reference)
+  {
+    && s.Ready?
+    && dop.NoDiskOp?
+
+    && IsAllocated(s, ref)
+
+    // We can only dealloc this if nothing is pointing to it.
+    && ref != G.Root()
+    && NoPredecessors(s.ephemeralIndirectionTable.graph, ref)
+
+    && s'.Ready?
+    && s'.persistentIndirectionTable == s.persistentIndirectionTable
+    && s'.ephemeralIndirectionTable.lbas == MapRemove(s.ephemeralIndirectionTable.lbas, {ref})
+    && s'.cache == MapRemove(s.cache, {ref})
+    && s'.ephemeralIndirectionTable.graph == MapRemove(s.ephemeralIndirectionTable.graph, {ref})
+  }
+
+  predicate PageInReq(k: Constants, s: Variables, s': Variables, dop: DiskOp, ref: Reference)
+  {
+    && s.Ready?
+    && dop.ReqReadOp?
+    && IsAllocated(s, ref)
+    && ref in s.ephemeralIndirectionTable.lbas
+    && ref !in s.cache
+    && s.ephemeralIndirectionTable.lbas[ref] == dop.reqRead.lba
+    && s' == s.(outstandingBlockReads := s.outstandingBlockReads[dop.id := OutstandingRead(ref)])
+  }
+}
+
